src/lib/kuiper/Kuiper.Conditional.fsti
@@ -5,6 +5,7 @@ module Kuiper.Conditional
 open Pulse.Lib.Pervasives
 open Pulse.Lib.BigStar
 
+[@@no_mkeys]
 let if_ (b: bool) (p: slprop): slprop = (cond b p emp)
 
 // REWRITE
